Start rewriting compute_memLogMap
These definitions are a huge pain to reason about, something must be
wrong with how I'm writing them.

src/program_proof/wal/highest.v
@@ -8,7 +8,9 @@ From Perennial.program_proof.wal Require Import specs.
 was formerly part of the Flush spec, and this kind of reasoning might be useful
 in the future. *)
 
-Implicit Types (pos:u64).
+Implicit Types (txn_id: nat) (pos: u64).
+(* everything in this file is about [nat]s *)
+Close Scope Z.
 
 (* NOTE: we no longer use [is_highest_txn] *)
 Definition is_highest_txn txns txn_id pos :=
@@ -23,12 +25,36 @@ Fixpoint find_highest_index poss pos: option nat :=
   | pos'::poss => if decide (pos = pos') then
                     (* if there's a higher index, use that one *)
                     match find_highest_index poss pos with
-                    | Some i => Some (1 + i)%nat
+                    | Some i => Some (1 + i)
                     (* otherwise, here is fine *)
-                    | None => Some 0%nat
+                    | None => Some 0
                     end
-                  else (λ i, (1 + i)%nat) <$> find_highest_index poss pos
+                  else (λ i, (1 + i)) <$> find_highest_index poss pos
   end.
+
+Fixpoint find_highest_index' poss pos: option nat :=
+  match poss with
+  | [] => None
+  | pos'::poss =>
+    let idx := (λ i, (1 + i)) <$> find_highest_index' poss pos in
+    match idx with
+    | Some _ => idx
+    | None => if (decide (pos = pos')) then Some 0 else None
+    end
+  end.
+
+Theorem find_highest_index'_ok poss pos :
+  find_highest_index poss pos = find_highest_index' poss pos.
+Proof.
+  induction poss; simpl; auto.
+  destruct (decide (pos = a)); auto.
+  - destruct_with_eqn (find_highest_index' poss pos); simpl; auto.
+    + rewrite IHposs //.
+    + rewrite IHposs //.
+  - destruct_with_eqn (find_highest_index poss pos); simpl; auto.
+    + rewrite -IHposs //.
+    + rewrite -IHposs //.
+Qed.
 
 Instance is_txn_dec txns txn_id pos : Decision (is_txn txns txn_id pos).
 Proof.
@@ -134,7 +160,7 @@ Qed.
 
 Theorem is_highest_txn_bound txns txn_id pos :
   is_highest_txn txns txn_id pos ->
-  (txn_id ≤ length txns)%nat.
+  txn_id ≤ length txns.
 Proof.
   destruct 1 as [His_txn _].
   eauto using is_txn_bound.
@@ -146,7 +172,7 @@ Lemma wal_wf_txns_mono_highest {σ txn_id1 pos1 txn_id2 pos2} :
   is_txn σ.(log_state.txns) txn_id1 pos1 ->
   is_highest_txn σ.(log_state.txns) txn_id2 pos2 ->
   int.val pos1 ≤ int.val pos2 ->
-  (txn_id1 ≤ txn_id2)%nat.
+  txn_id1 ≤ txn_id2.
 Proof.
   intros Hwf Htxn1 Htxn2 Hle.
   destruct (decide (pos1 = pos2)); subst.
@@ -159,3 +185,79 @@ Proof.
       lia.
 Qed.
 *)
+
+Fixpoint pos_indices (poss: list u64) (i: nat): gmap u64 nat :=
+  match poss with
+  | [] => ∅
+  | pos::poss =>
+    let m := pos_indices poss (S i) in
+    match m !! pos with
+    | Some _ => m
+    | None => <[pos := i]> m
+    end
+  end.
+
+Theorem option_Some_eq {A} (x1 x2: A) :
+  Some x1 = Some x2 <-> x1 = x2.
+Proof.
+  split; congruence.
+Qed.
+
+Theorem find_highest_index_none_pos_indices poss pos i0 :
+  find_highest_index poss pos = None <->
+  pos_indices poss i0 !! pos = None.
+Proof.
+  revert i0 pos.
+  induction poss; simpl; intros i0 pos.
+  - rewrite lookup_empty //.
+  - destruct (decide (pos = a)); subst.
+    { destruct (find_highest_index poss a);
+        (split; [ congruence | ]).
+      - destruct_with_eqn (pos_indices poss (S i0) !! a); try congruence.
+        rewrite lookup_insert //.
+      - destruct_with_eqn (pos_indices poss (S i0) !! a); try congruence.
+        rewrite lookup_insert //.
+    }
+    rewrite fmap_None.
+    rewrite (IHposs (S i0)).
+    { split; intros H.
+      - destruct_with_eqn (pos_indices poss (S i0) !! a); try congruence.
+        rewrite -> lookup_insert_ne by auto; auto.
+      - destruct_with_eqn (pos_indices poss (S i0) !! a); try congruence.
+        rewrite -> lookup_insert_ne in H by auto; auto.
+    }
+Qed.
+
+Lemma pos_indices_fmap_highest (poss: list u64) (i0: nat) :
+  forall pos,
+    (λ i, i0 + i) <$> find_highest_index poss pos =
+    pos_indices poss i0 !! pos.
+Proof.
+  setoid_rewrite find_highest_index'_ok.
+  revert i0.
+  induction poss; simpl; intros i0 pos.
+  - rewrite lookup_empty; split; congruence.
+  - setoid_rewrite <- IHposs.
+    destruct (decide (pos = a)); subst.
+    + destruct (find_highest_index' poss a) eqn:Hidx; simpl.
+      * rewrite -IHposs Hidx /=; auto.
+      * rewrite lookup_insert; auto.
+    + destruct (find_highest_index' poss pos) eqn:Hidx; simpl.
+      * destruct (find_highest_index' poss a) eqn:Hidx'; simpl.
+        { rewrite -IHposs Hidx /=; auto. }
+        rewrite -> lookup_insert_ne by auto.
+        rewrite -IHposs Hidx /=; auto.
+      * destruct (find_highest_index' poss a) eqn:Hidx'; simpl.
+        { rewrite -IHposs Hidx /=; auto. }
+        rewrite -> lookup_insert_ne by auto.
+        rewrite -IHposs Hidx /=; auto.
+Qed.
+
+Theorem pos_indices_lookup (poss: list u64) :
+  forall pos,
+    pos_indices poss 0 !! pos = find_highest_index poss pos.
+Proof.
+  intros.
+  rewrite -pos_indices_fmap_highest.
+  destruct (find_highest_index poss pos); auto.
+Qed.
