src/program_proof/wal/read_proof.v
@@ -19,8 +19,7 @@ Let circN := walN .@ "circ".
 
 Lemma memLogMap_ok_memLog_lookup memStart memLog a i :
   int.val memStart + Z.of_nat (length memLog) < 2^64 ->
-  map_get (compute_memLogMap memLog memStart ∅) a
-  = (i, true) ->
+  map_get (compute_memLogMap memLog memStart ∅) a = (i, true) ->
   ∃ b, memLog !! int.nat (word.sub i memStart) = Some (update.mk a b)
   (* also, i is the highest index such that this is true *).
 Proof.
